cp

vale/specs/interop/Interop.X64.fsti
@@ -209,17 +209,31 @@ let create_initial_trusted_state (args:arity_ok arg)
 ////////////////////////////////////////////////////////////////////////////////
 let stack_buffer = lowstar_buffer (ME.TBase ME.TUInt64)
 
+let prediction_pre_rel_t (c:TS.tainted_code) (args:arity_ok arg) =
+    h0:mem_roots args ->
+    prop
+
+let prediction_post_rel_t (c:TS.tainted_code) (args:arity_ok arg) =
+    h0:mem_roots args ->
+    s0:TS.traceState ->
+    push_h0:mem_roots args ->
+    alloc_push_h0:mem_roots args ->
+    b:stack_buffer{mem_roots_p alloc_push_h0 (arg_of_b8 b::args)} ->
+    (nat & ME.mem) ->
+    sn:TS.traceState ->
+    prop
+
 let prediction_pre
-    (pre_rel: (args:arity_ok arg -> mem_roots args -> prop))
     (c:TS.tainted_code)
     (args:arity_ok arg)
+    (pre_rel: prediction_pre_rel_t c args)
     (h0:mem_roots args)
     (s0:TS.traceState)
     (push_h0:mem_roots args)
     (alloc_push_h0:mem_roots args)
     (b:stack_buffer{mem_roots_p alloc_push_h0 (arg_of_b8 b::args)})
     =
-  pre_rel args h0 /\
+  pre_rel h0 /\
   HS.fresh_frame h0 push_h0 /\
   B.modifies B.loc_none push_h0 alloc_push_h0 /\
   HS.get_tip push_h0 == HS.get_tip alloc_push_h0 /\
@@ -228,9 +242,9 @@ let prediction_pre
   s0 == fst (create_initial_trusted_state args alloc_push_h0 b)
 
 let prediction_post
-    (post_rel: (nat & ME.mem) -> TS.traceState -> prop)
     (c:TS.tainted_code)
     (args:arity_ok arg)
+    (post_rel: prediction_post_rel_t c args)
     (h0:mem_roots args)
     (s0:TS.traceState)
     (push_h0:mem_roots args)
@@ -246,41 +260,24 @@ let prediction_post
     IM.down_mem h1 (IA.addrs)
                 (Adapters.ptrs_of_mem final_mem) == s1.TS.state.BS.mem /\
     calling_conventions s0 s1 /\
-    post_rel fuel_mem s1
+    post_rel h0 s0 push_h0 alloc_push_h0 b fuel_mem s1
   )
 
 
-let prediction_pre_rel_t =
-    c:TS.tainted_code ->
-    args:arity_ok arg ->
-    h0:mem_roots args ->
-    prop
-
-let prediction_post_rel_t =
-    c:TS.tainted_code ->
-    args:arity_ok arg ->
-    h0:mem_roots args ->
-    s0:TS.traceState ->
-    push_h0:mem_roots args ->
-    alloc_push_h0:mem_roots args ->
-    b:stack_buffer{mem_roots_p alloc_push_h0 (arg_of_b8 b::args)} ->
-    (nat & ME.mem) ->
-    sn:TS.traceState ->
-    prop
 
 let prediction
-    (pre_rel:prediction_pre_rel_t)
-    (post_rel:prediction_post_rel_t)
     (c:TS.tainted_code)
-    (args:arity_ok arg) =
-  h0:mem_roots args{pre_rel c args h0} ->
+    (args:arity_ok arg)
+    (pre_rel:prediction_pre_rel_t c args)
+    (post_rel:prediction_post_rel_t c args) =
+  h0:mem_roots args{pre_rel h0} ->
   s0:TS.traceState ->
   push_h0:mem_roots args ->
   alloc_push_h0:mem_roots args ->
   b:stack_buffer{mem_roots_p h0 args /\ mem_roots_p alloc_push_h0 (arg_of_b8 b::args)} ->
   Ghost (nat & ME.mem)
-    (requires prediction_pre (pre_rel c) c args h0 s0 push_h0 alloc_push_h0 b)
-    (ensures prediction_post (post_rel c args h0 s0 push_h0 alloc_push_h0 b) c args h0 s0 push_h0 alloc_push_h0 b)
+    (requires prediction_pre c args pre_rel h0 s0 push_h0 alloc_push_h0 b)
+    (ensures prediction_post c args post_rel h0 s0 push_h0 alloc_push_h0 b)
 
 noeq type as_lowstar_sig_ret (args:arity_ok arg) =
   | As_lowstar_sig_ret :
@@ -297,13 +294,13 @@ let as_lowstar_sig_post
     (h0:mem_roots args)
     (#pre_rel:_)
     (#post_rel: _)
-    (predict:prediction pre_rel post_rel c args)
+    (predict:prediction c args pre_rel post_rel)
     (ret:as_lowstar_sig_ret args)
     (h1:HS.mem) =
   let As_lowstar_sig_ret push_h0 alloc_push_h0 b fuel final_mem = ret in
   let s0 = fst (create_initial_trusted_state args alloc_push_h0 b) in
   let pre_pop = Adapters.hs_of_mem final_mem in
-  prediction_pre (pre_rel c) c args h0 s0 push_h0 alloc_push_h0 b /\
+  prediction_pre c args pre_rel h0 s0 push_h0 alloc_push_h0 b /\
   (fuel, final_mem) == predict h0 s0 push_h0 alloc_push_h0 b /\
   FStar.HyperStack.ST.equal_domains alloc_push_h0 pre_pop /\
   HS.poppable pre_pop /\
@@ -314,9 +311,9 @@ let as_lowstar_sig (c:TS.tainted_code) =
 //    h0:mem_roots args ->
     #pre_rel:_ ->
     #post_rel:_ ->
-    predict:prediction pre_rel post_rel c args ->
+    predict:prediction c args pre_rel post_rel ->
     FStar.HyperStack.ST.Stack (as_lowstar_sig_ret args)
-        (requires (fun h0 -> mem_roots_p h0 args /\ pre_rel c args h0))
+        (requires (fun h0 -> mem_roots_p h0 args /\ pre_rel h0))
         (ensures fun h0 ret h1 -> as_lowstar_sig_post c args h0 predict ret h1)
 
 val wrap_variadic (c:TS.tainted_code) : as_lowstar_sig c
@@ -324,19 +321,47 @@ val wrap_variadic (c:TS.tainted_code) : as_lowstar_sig c
 let (++) (#t:td) (x:td_as_type t) (args:list arg) = (| t, x |) :: args
 module List = FStar.List.Tot
 
+let arity_ok_2 (l:list 'a) (m:list 'b) = List.length l + List.length m < max_arity
+
+let rec rel_gen_t
+      (c:TS.tainted_code)
+      (td:list td)
+      (args:list arg{arity_ok_2 td args})
+      (f: arity_ok arg -> Type) =
+    match td with
+    | [] -> f args
+    | hd::tl ->
+      x:td_as_type hd ->
+      rel_gen_t c tl (x++args) f
+
+let elim_rel_gen_t_nil #c #args #f (x:rel_gen_t c [] args f)
+  : f args
+  = x
+
+let elim_rel_gen_t_cons #c hd tl #args #f (p:rel_gen_t c (hd::tl) args f)
+  : (x:td_as_type hd ->
+      rel_gen_t c tl (x++args) f)
+  = p
+
+
 let rec prediction_t
       (c:TS.tainted_code)
       (dom:list td)
       (args:list arg{List.length dom + List.length args < max_arity})
-      (pre_rel:_)
-      (post_rel:_)
+      (pre_rel:rel_gen_t c dom args (prediction_pre_rel_t c))
+      (post_rel:rel_gen_t c dom args (prediction_post_rel_t c))
     = match dom with
       | [] ->
-        prediction pre_rel post_rel c args
+        prediction c args pre_rel post_rel
 
       | hd::tl ->
         x:td_as_type hd ->
-        prediction_t c tl (x ++ args) pre_rel post_rel
+        prediction_t
+          c
+          tl
+          (x ++ args)
+          (elim_rel_gen_t_cons hd tl pre_rel x)
+          (elim_rel_gen_t_cons hd tl post_rel x)
 
 let elim_predict_t_nil
       (#c:TS.tainted_code)
@@ -344,34 +369,36 @@ let elim_predict_t_nil
       (#pre_rel:_)
       (#post_rel:_)
       (p:prediction_t c [] args pre_rel post_rel)
-   : prediction pre_rel post_rel c args
+   : prediction c args pre_rel post_rel
    = p
 
 let elim_predict_t_cons
       (#c:TS.tainted_code)
       (hd:td)
       (tl:list td)
-      (#args:list arg{List.length (hd::tl) + List.length args < max_arity})
+      (#args:list arg{arity_ok_2 (hd::tl) args})
       (#pre_rel:_)
       (#post_rel:_)
       (p:prediction_t c (hd::tl) args pre_rel post_rel)
    : x:td_as_type hd ->
-     prediction_t c tl (x ++ args) pre_rel post_rel
+     prediction_t c tl (x ++ args)
+       (elim_rel_gen_t_cons hd tl pre_rel x)
+       (elim_rel_gen_t_cons hd tl post_rel x)
    = p
 
 let rec as_lowstar_sig_t
       (c:TS.tainted_code)
       (dom:list td)
       (args:list arg{List.length dom + List.length args < max_arity})
-      (#pre_rel:_)
-      (#post_rel:_)
+      (pre_rel:rel_gen_t c dom args (prediction_pre_rel_t c))
+      (post_rel:rel_gen_t c dom args (prediction_post_rel_t c))
       // (#h0:HS.mem)
       (predict:prediction_t c dom args pre_rel post_rel) =
       match dom with
       | [] ->
         (unit ->
          FStar.HyperStack.ST.Stack (as_lowstar_sig_ret args)
-           (requires (fun h0 -> mem_roots_p h0 args /\ pre_rel c args h0))
+           (requires (fun h0 -> mem_roots_p h0 args /\ (elim_rel_gen_t_nil pre_rel h0)))
            (ensures fun h0 ret h1 -> as_lowstar_sig_post c args h0 #pre_rel #post_rel (elim_predict_t_nil predict) ret h1))
       | hd::tl ->
         x:td_as_type hd ->
@@ -379,12 +406,14 @@ let rec as_lowstar_sig_t
           c
           tl
           (x ++ args)
+          (elim_rel_gen_t_cons hd tl pre_rel x)
+          (elim_rel_gen_t_cons hd tl post_rel x)
           (elim_predict_t_cons hd tl predict x)
 
 val wrap
     (c:TS.tainted_code)
     (dom:arity_ok td)
-    (#pre_rel:_)
-    (#post_rel:_)
+    (#pre_rel:rel_gen_t c dom [] (prediction_pre_rel_t c))
+    (#post_rel:rel_gen_t c dom [] (prediction_post_rel_t c))
     (predict:prediction_t c dom [] pre_rel post_rel)
-  : as_lowstar_sig_t c dom [] predict
+  : as_lowstar_sig_t c dom [] pre_rel post_rel predict
