vale/specs/interop/Interop.X64.fst
@@ -48,22 +48,26 @@ let rec wrap_aux
     (c:TS.tainted_code)
     (dom:list td)
     (args:list arg{List.length dom + List.length args < max_arity})
-    (#pre_rel:_)
-    (#post_rel:_)
+    (pre_rel:rel_gen_t c dom args (prediction_pre_rel_t c))
+    (post_rel:rel_gen_t c dom args (prediction_post_rel_t c))
     (predict:prediction_t c dom args pre_rel post_rel)
-  : as_lowstar_sig_t c dom args predict
+  : as_lowstar_sig_t c dom args pre_rel post_rel predict
   = match dom with
     | [] ->
       let f () :
         FStar.HyperStack.ST.Stack (as_lowstar_sig_ret args)
-           (requires (fun h0 -> mem_roots_p h0 args /\ pre_rel c args h0))
+           (requires (fun h0 -> mem_roots_p h0 args /\ elim_rel_gen_t_nil pre_rel h0))
            (ensures fun h0 ret h1 -> as_lowstar_sig_post c args h0 #pre_rel #post_rel (elim_predict_t_nil predict) ret h1) =
         wrap_variadic c args (elim_predict_t_nil predict)
       in
-      f <: as_lowstar_sig_t c [] args predict
+      f <: as_lowstar_sig_t c [] args pre_rel post_rel predict
 
     | hd::tl ->
       fun (x:td_as_type hd) ->
-      wrap_aux c tl (x ++ args) (elim_predict_t_cons hd tl predict x)
+      wrap_aux c tl
+        (x ++ args)
+        (elim_rel_gen_t_cons hd tl pre_rel x)
+        (elim_rel_gen_t_cons hd tl post_rel x)
+        (elim_predict_t_cons hd tl predict x)
 
-let wrap c dom = wrap_aux c dom []
+let wrap c dom #pre_rel #post_rel predict = wrap_aux c dom [] pre_rel post_rel predict
